SPHINCS_PLUS_TW.ec
@@ -8,7 +8,7 @@ require import AllCore List Distr IntDiv RealExp StdOrder FinType BitEncoding.
 require import BinaryTrees MerkleTrees.
 require (*--*) KeyedHashFunctions TweakableHashFunctions HashAddresses.
 require (*--*) DigitalSignatures.
-require (*--*) FORS_TW_ES FL_XMSS_MT_TW_ES.
+require (*--*) FORS_TW_ES FL_SL_XMSS_MT_TW_ES.
 
 
 
@@ -518,11 +518,17 @@ op set_lidx (ad : adrs) (i : int) : adrs =
 op set_tidx (ad : adrs) (i : int) : adrs =
   set_idx ad 4 i.
 
+op set_ltidx (ad : adrs) (i j : int) : adrs =
+  insubd (put (put (val ad) 4 j) 5 i).
+
 op set_typeidx (ad : adrs) (i : int) : adrs =
   insubd (put (put (put (put (val ad) 0 0) 1 0) 2 0) 3 i).
   
 op set_kpidx (ad : adrs) (i : int) : adrs =
   set_idx ad 2 i.
+
+op set_thtbidx (ad : adrs) (i j : int) : adrs =
+  insubd (put (put (val ad) 0 j) 1 i).
 
 
 (* -- Keyed hash functions -- *)
@@ -634,6 +640,7 @@ clone import FORS_TW_ES as FTWES with
     op set_tidx <- set_tidx,
     op set_typeidx <- set_typeidx,
     op set_kpidx <- set_kpidx,
+    op set_thtbidx <- set_thtbidx,
     
     op skg <- skg,
     op mkg <- mkg,
@@ -682,8 +689,8 @@ clone import FORS_TW_ES as FTWES with
 import DBAL BLKAL DBAPKL DBLLKTL.
 
 
-(* FL-XMSS-MT-TW *)
-clone import FL_XMSS_MT_TW_ES as FXMTWES with
+(* FL-SL-XMSS-MT-TW *)
+clone import FL_SL_XMSS_MT_TW_ES as FSXMTWES with
     op adrs_len <- adrs_len,
     op n <- n,
     op log2_w <- log2_w,
@@ -718,13 +725,16 @@ clone import FL_XMSS_MT_TW_ES as FXMTWES with
     
     op set_lidx <- set_lidx,
     op set_tidx <- set_tidx,
+    op set_ltidx <- set_ltidx,
     op set_typeidx <- set_typeidx,
     op set_kpidx <- set_kpidx,
+    op set_thtbidx <- set_thtbidx,
     
     op thfc <- thfc,
     op trh <- trh,
     op pkco <- pkco,
     op WTWES.f <- f,
+    op WTWES.skg <- skg,
     
     op dpseed <- dpseed,
     op ddgstblock <- ddgstblock,
@@ -777,7 +787,7 @@ type pkSPHINCSPLUSTW = dgstblock * pseed.
 type skSPHINCSPLUSTW = mseed * sseed * pseed.
 
 (* Signatures *)
-type sigSPHINCSPLUSTW = mkey * sigFORS * sigFLXMSSMTNI. 
+type sigSPHINCSPLUSTW = mkey * sigFORSTW * sigFLSLXMSSMTTW. 
 
 
 
@@ -805,13 +815,13 @@ module SPHINCS_PLUS_TW : Scheme = {
     var pk : pkSPHINCSPLUSTW;
     var sk : skSPHINCSPLUSTW;
     
-    ad <- witness;
+    ad <- insubd [0; 0; chtype; 0; 0; 0];
     
     ms <$ dmseed;
     ss <$ dsseed;
     
     ps <$ dpseed;
-    root <@ FL_XMSS_MT_TW_ES.gen_root(ss, ps, ad);
+    root <@ FL_SL_XMSS_MT_TW_ES.gen_root(ss, ps, ad);
     
     pk <- (root, ps);
     sk <- (ms, ss, ps);
@@ -825,19 +835,19 @@ module SPHINCS_PLUS_TW : Scheme = {
     var ps : pseed;
     var ad : adrs;
     var mk : mkey;
-    var sigFORS : sigFORS;
-    var cm : msgFORS;
+    var sigFORSTW : sigFORSTW;
+    var cm : msgFORSTW;
     var idx : index;
     var tidx, kpidx : int;
     var pkFORS : pkFORS;
-    var sigFLXMSSMTNI : sigFLXMSSMTNI;
+    var sigFLSLXMSSMTTW : sigFLSLXMSSMTTW;
     var sig : sigSPHINCSPLUSTW;
         
     (ms, ss, ps) <- sk;
     
-    ad <- witness;
+    ad <- insubd [0; 0; chtype; 0; 0; 0];
     
-    (mk, sigFORS) <@ M_FORS_TW_ES.sign((ms, ss, ps, set_lidx ad 0), m);
+    (mk, sigFORSTW) <@ M_FORS_TW_ES.sign((ms, ss, ps, ad), m);
     
     (cm, idx) <- mco mk m;
     
@@ -845,35 +855,35 @@ module SPHINCS_PLUS_TW : Scheme = {
     
     pkFORS <@ FL_FORS_TW_ES.gen_pkFORS(ss, ps, set_kpidx (set_tidx (set_typeidx (set_lidx ad 0) trhftype) tidx) kpidx);
     
-    (idx, sigFLXMSSMTNI) <@ FL_XMSS_MT_TW_ES.sign((idx, ss, ps, ad), pkFORS);
+    sigFLSLXMSSMTTW <@ FL_SL_XMSS_MT_TW_ES.sign((ss, ps, ad), pkFORS, idx);
     
-    return (mk, sigFORS, sigFLXMSSMTNI);
+    return (mk, sigFORSTW, sigFLSLXMSSMTTW);
   }
   
   proc verify(pk : pkSPHINCSPLUSTW, m : msg, sig : sigSPHINCSPLUSTW) : bool = {
     var root, root' : dgstblock;
     var ps : pseed;
     var mk : mkey;
-    var sigFORS : sigFORS;
-    var sigFLXMSSMTNI : sigFLXMSSMTNI;
+    var sigFORSTW : sigFORSTW;
+    var sigFLSLXMSSMTTW : sigFLSLXMSSMTTW;
     var ad : adrs;
-    var cm : msgFORS;
+    var cm : msgFORSTW;
     var idx : index;
     var tidx, kpidx : int;
     var pkFORS : pkFORS;
     
     (root, ps) <- pk;
-    (mk, sigFORS, sigFLXMSSMTNI) <- sig;
+    (mk, sigFORSTW, sigFLSLXMSSMTTW) <- sig;
     
-    ad <- witness;
+    ad <- insubd [0; 0; chtype; 0; 0; 0];
     
     (cm, idx) <- mco mk m;
     
     (tidx, kpidx) <- edivz (val idx) l';
     
-    pkFORS <@ FL_FORS_TW_ES.pkFORS_from_sigFORS(sigFORS, cm, ps, set_kpidx (set_tidx (set_typeidx (set_lidx ad 0) trhftype) tidx) kpidx);
+    pkFORS <@ FL_FORS_TW_ES.pkFORS_from_sigFORSTW(sigFORSTW, cm, ps, set_kpidx (set_tidx (set_typeidx (set_lidx ad 0) trhftype) tidx) kpidx);
     
-    root' <@ FL_XMSS_MT_TW_ES.root_from_sigFLXMSSMTTW(pkFORS, (idx, sigFLXMSSMTNI), ps, ad);
+    root' <@ FL_SL_XMSS_MT_TW_ES.root_from_sigFLSLXMSSMTTW(pkFORS, sigFLSLXMSSMTTW, idx, ps, ad);
     
     return root' = root;
   }
@@ -883,23 +893,336 @@ module SPHINCS_PLUS_TW : Scheme = {
 
 (* - Proof - *)
 (* -- Reduction adversaries -- *)
-module R_MFORSTWESEUFCMA_EUFCMA (A : Adv_EUFCMA) = {
-
+module (R_SKGPRF_EUFCMA (A : Adv_EUFCMA) : SKG_PRF.Adv_PRF) (O : SKG_PRF.Oracle_PRF) = {
+  proc distinguish() : bool = {
+    
+    return witness;
+  }
 }.
 
-module R_FLXMSSMTTWESEUFNACMA_EUFCMA (A : Adv_EUFCMA) = {
+module (R_MKGPRF_EUFCMA (A : Adv_EUFCMA) : MKG_PRF.Adv_PRF) (O : MKG_PRF.Oracle_PRF) = {
+  proc distinguish() : bool = {
+    return witness;
+  }
+}.
 
+module (R_MFORSTWESNPRFEUFCMA_EUFCMA (A : Adv_EUFCMA) : Adv_EUFCMA_MFORSTWESNPRF) (O : SOracle_CMA_MFORSTWESNPRF) = {
+  proc forge(pk : pkFORS list list * pseed * adrs) : msg * (mkey * sigFORSTW) = {
+    return witness;
+  }
+}.
+
+module R_FLSLXMSSMTTWESNPRFEUFNACMA_EUFCMA (A : Adv_EUFCMA) : Adv_EUFNACMA_FLSLXMSSMTTWESNPRF = {
+  proc choose(pk : pkFLSLXMSSMTTW) : msgFLSLXMSSMTTW list = {
+    return witness;
+  }
+  
+  proc forge(sigl : sigFLSLXMSSMTTW list) : msgFLSLXMSSMTTW * sigFLSLXMSSMTTW * index = {
+    return witness;
+  }
 }.
 
 
 section Proof_SPHINCS_PLUS_TW_EUFCMA.
 
+local module SPHINCS_PLUS_TW_Aux = {
+  proc keygen_prf() : pkSPHINCSPLUSTW * (skFORS list list * skWOTS list list list * pseed) = {
+    var ad : adrs;
+    var ms : mseed;
+    var ss : sseed;
+    var ps : pseed;
+    var skFORS_ele : dgstblock;
+    var skFORSet : dgstblock list;
+    var skFORS : dgstblock list list;
+    var skFORSlp : skFORS list; 
+    var skFORSnt : skFORS list list;
+    var skWOTS_ele : dgstblock;
+    var skWOTS : dgstblock list;
+    var skWOTSlp : skWOTS list;
+    var skWOTSnt : skWOTS list list;
+    var skWOTStd : skWOTS list list list;
+    var leaves : dgstblock list;
+    var root : dgstblock;
+    var pk : pkSPHINCSPLUSTW;
+    var sk : skFORS list list * skWOTS list list list * pseed;
+    
+    ad <- insubd [0; 0; chtype; 0; 0; 0];
+    
+    ms <$ dmseed;
+    ss <$ dsseed;
+    
+    ps <$ dpseed;
+    
+    
+    skFORSnt <- [];
+    while (size skFORSnt < nr_trees 0) {
+      skFORSlp <- [];
+      while (size skFORSlp < l') {
+         skFORS <- [];
+         while (size skFORS < k) {
+          skFORSet <- [];
+          while (size skFORSet < t) {
+            skFORS_ele <- skg ss (ps, set_thtbidx (set_kpidx (set_tidx (set_typeidx ad trhftype) (size skFORSnt)) (size skFORSlp)) 0 (size skFORS * t + size skFORSet));
+            skFORSet <- rcons skFORSet skFORS_ele;
+          }
+          skFORS <- rcons skFORS skFORSet;  
+        }
+        skFORSlp <- rcons skFORSlp (insubd skFORS);  
+      }
+      skFORSnt <- rcons skFORSnt skFORSlp;
+    }
+    
+    skWOTStd <- [];
+    while (size skWOTStd < d) {
+      skWOTSnt <- [];
+      while (size skWOTSnt < nr_trees (size skWOTStd)) {
+        skWOTSlp <- [];
+        while (size skWOTSlp < l') {
+          skWOTS <- [];
+          while (size skWOTS < len) {
+            skWOTS_ele <- skg ss (ps, set_hidx (set_chidx (set_kpidx (set_typeidx (set_ltidx ad (size skWOTStd) (size skWOTSnt)) chtype) (size skWOTSlp)) (size skWOTS)) 0);
+            skWOTS <- rcons skWOTS skWOTS_ele;  
+          }
+          
+          (* Add WOTS-TW secret key to list of secret keys of this inner tree *)
+          skWOTSlp <- rcons skWOTSlp (DBLL.insubd skWOTS);
+        }
+        
+        (* Add secret key of inner tree to list of secret keys in this layer *)
+        skWOTSnt <- rcons skWOTSnt skWOTSlp;
+      }
+      (* Add secret key of layer to list of secret keys for all layers *)
+      skWOTStd <- rcons skWOTStd skWOTSnt; 
+    }
+
+    (* 
+      Extract secret key of the top-most inner tree in the hyper tree 
+      and compute the corresponding leaves.
+    *)
+    skWOTSlp <- nth witness (nth witness skWOTStd (d - 1)) 0;
+    leaves <@ FL_SL_XMSS_MT_TW_ES_NPRF.leaves_from_sklpsad(skWOTSlp, ps, set_ltidx ad (d - 1) 0);
+    
+    (*
+      Compute root (hash value) from the computed list of leaves, given public seed, and
+      given address (after setting the type to tree hashing)
+    *)
+    root <- val_bt_trh ps (set_typeidx (set_ltidx ad (d - 1) 0) trhxtype) (list2tree leaves) h' 0;
+    
+    pk <- (root, ps);
+    sk <- (skFORSnt, skWOTStd, ps);
+
+    return (pk, sk);
+  }
+
+  proc keygen_nprf() : pkSPHINCSPLUSTW * (skFORS list list * skWOTS list list list * pseed) = {
+    var ad : adrs;
+    var ms : mseed;
+    var ss : sseed;
+    var ps : pseed;
+    var skFORS_ele : dgstblock;
+    var skFORSet : dgstblock list;
+    var skFORS : dgstblock list list;
+    var skFORSlp : skFORS list; 
+    var skFORSnt : skFORS list list;
+    var skWOTS_ele : dgstblock;
+    var skWOTS : dgstblock list;
+    var skWOTSlp : skWOTS list;
+    var skWOTSnt : skWOTS list list;
+    var skWOTStd : skWOTS list list list;
+    var leaves : dgstblock list;
+    var root : dgstblock;
+    var pk : pkSPHINCSPLUSTW;
+    var sk : skFORS list list * skWOTS list list list * pseed;
+    
+    ad <- insubd [0; 0; chtype; 0; 0; 0];
+    
+    ms <$ dmseed;
+    ss <$ dsseed;
+    
+    ps <$ dpseed;
+    
+    
+    skFORSnt <- [];
+    while (size skFORSnt < nr_trees 0) {
+      skFORSlp <- [];
+      while (size skFORSlp < l') {
+         skFORS <- [];
+         while (size skFORS < k) {
+          skFORSet <- [];
+          while (size skFORSet < t) {
+            skFORS_ele <$ ddgstblock;
+            skFORSet <- rcons skFORSet skFORS_ele;
+          }
+          skFORS <- rcons skFORS skFORSet;  
+        }
+        skFORSlp <- rcons skFORSlp (insubd skFORS);  
+      }
+      skFORSnt <- rcons skFORSnt skFORSlp;
+    }
+    
+    skWOTStd <- [];
+    while (size skWOTStd < d) {
+      skWOTSnt <- [];
+      while (size skWOTSnt < nr_trees (size skWOTStd)) {
+        skWOTSlp <- [];
+        while (size skWOTSlp < l') {
+          skWOTS <- [];
+          while (size skWOTS < len) {
+            skWOTS_ele <$ ddgstblock;
+            skWOTS <- rcons skWOTS skWOTS_ele;  
+          }
+          
+          (* Add WOTS-TW secret key to list of secret keys of this inner tree *)
+          skWOTSlp <- rcons skWOTSlp (DBLL.insubd skWOTS);
+        }
+        
+        (* Add secret key of inner tree to list of secret keys in this layer *)
+        skWOTSnt <- rcons skWOTSnt skWOTSlp;
+      }
+      (* Add secret key of layer to list of secret keys for all layers *)
+      skWOTStd <- rcons skWOTStd skWOTSnt; 
+    }
+
+    (* 
+      Extract secret key of the top-most inner tree in the hyper tree 
+      and compute the corresponding leaves.
+    *)
+    skWOTSlp <- nth witness (nth witness skWOTStd (d - 1)) 0;
+    leaves <@ FL_SL_XMSS_MT_TW_ES_NPRF.leaves_from_sklpsad(skWOTSlp, ps, set_ltidx ad (d - 1) 0);
+    
+    (*
+      Compute root (hash value) from the computed list of leaves, given public seed, and
+      given address (after setting the type to tree hashing)
+    *)
+    root <- val_bt_trh ps (set_typeidx (set_ltidx ad (d - 1) 0) trhxtype) (list2tree leaves) h' 0;
+    
+    pk <- (root, ps);
+    sk <- (skFORSnt, skWOTStd, ps);
+
+    return (pk, sk);
+  }
+    
+  proc sign(sk : skSPHINCSPLUSTW, m : msg) : sigSPHINCSPLUSTW = {
+    var ms : mseed;
+    var ss : sseed;
+    var ps : pseed;
+    var ad : adrs;
+    var mk : mkey;
+    var sigFORSTW : sigFORSTW;
+    var cm : msgFORSTW;
+    var idx : index;
+    var tidx, kpidx : int;
+    var pkFORS : pkFORS;
+    var sigFLSLXMSSMTTW : sigFLSLXMSSMTTW;
+    var sig : sigSPHINCSPLUSTW;
+        
+    (ms, ss, ps) <- sk;
+    
+    ad <- witness;
+    
+    (mk, sigFORSTW) <@ M_FORS_TW_ES.sign((ms, ss, ps, set_lidx ad 0), m);
+    
+    (cm, idx) <- mco mk m;
+    
+    (tidx, kpidx) <- edivz (val idx) l';
+    
+    pkFORS <@ FL_FORS_TW_ES.gen_pkFORS(ss, ps, set_kpidx (set_tidx (set_typeidx (set_lidx ad 0) trhftype) tidx) kpidx);
+    
+    sigFLSLXMSSMTTW <@ FL_SL_XMSS_MT_TW_ES.sign((ss, ps, ad), pkFORS, idx);
+    
+    return (mk, sigFORSTW, sigFLSLXMSSMTTW);
+  }
+  
+  proc verify(pk : pkSPHINCSPLUSTW, m : msg, sig : sigSPHINCSPLUSTW) : bool = {
+    var root, root' : dgstblock;
+    var ps : pseed;
+    var mk : mkey;
+    var sigFORSTW : sigFORSTW;
+    var sigFLSLXMSSMTTW : sigFLSLXMSSMTTW;
+    var ad : adrs;
+    var cm : msgFORSTW;
+    var idx : index;
+    var tidx, kpidx : int;
+    var pkFORS : pkFORS;
+    
+    (root, ps) <- pk;
+    (mk, sigFORSTW, sigFLSLXMSSMTTW) <- sig;
+    
+    ad <- witness;
+    
+    (cm, idx) <- mco mk m;
+    
+    (tidx, kpidx) <- edivz (val idx) l';
+    
+    pkFORS <@ FL_FORS_TW_ES.pkFORS_from_sigFORSTW(sigFORSTW, cm, ps, set_kpidx (set_tidx (set_typeidx (set_lidx ad 0) trhftype) tidx) kpidx);
+    
+    root' <@ FL_SL_XMSS_MT_TW_ES.root_from_sigFLSLXMSSMTTW(pkFORS, sigFLSLXMSSMTTW, idx, ps, ad);
+    
+    return root' = root;
+  }
+}.
+
 declare module A <: Adv_EUFCMA {}.
 
+
+(* 
+  Proof functional equivalence between original SPHINCS_PLUS_TW and a variant that immediately generates all
+  necessary secret values (for both the FORS and XMSS-MT parts) and maintains this collection of secret values 
+  throughout, pulling the desired secret values from this collection when neeeded (instead of regenerating them via
+  skg).  
+*)
+
+(*
+  Define variant that 
+*)
+
+
+
+local lemma EUFCMA_SPHINCS_PLUS_TW_FX &m :
+  Pr[EUF_CMA(SPHINCS_PLUS_TW, A, O_CMA_Default).main() @ &m : res]
+  <= 
+  `|  Pr[MKG_PRF.PRF(R_MKGPRF_EUFCMA(A), MKG_PRF.O_PRF_Default).main(true) @ &m : res]
+    - Pr[MKG_PRF.PRF(R_MKGPRF_EUFCMA(A), MKG_PRF.O_PRF_Default).main(false) @ &m : res] |
+  +
+  `|  Pr[SKG_PRF.PRF(R_SKGPRF_EUFCMA(A), SKG_PRF.O_PRF_Default).main(true) @ &m : res]
+    - Pr[SKG_PRF.PRF(R_SKGPRF_EUFCMA(A), SKG_PRF.O_PRF_Default).main(false) @ &m : res] |
+  +  
+  Pr[EUF_CMA_MFORSTWESNPRF(R_MFORSTWESNPRFEUFCMA_EUFCMA(A), O_CMA_MFORSTWESNPRF).main() @ &m : res]
+  +
+  Pr[EUF_NACMA_FLSLXMSSMTTWESNPRF(R_FLSLXMSSMTTWESNPRFEUFNACMA_EUFCMA(A)).main() @ &m : res].
+proof. admit. qed.
+
+(* TODO: replace OpenPRE by DSPR and TCR *)
 lemma EUFCMA_SPHINCS_PLUS_TW &m :
   Pr[EUF_CMA(SPHINCS_PLUS_TW, A, O_CMA_Default).main() @ &m : res]
   <= 
-  witness.
+  `|  Pr[MKG_PRF.PRF(R_MKGPRF_EUFCMA(A), MKG_PRF.O_PRF_Default).main(true) @ &m : res]
+    - Pr[MKG_PRF.PRF(R_MKGPRF_EUFCMA(A), MKG_PRF.O_PRF_Default).main(false) @ &m : res] |
+  +
+  `|  Pr[SKG_PRF.PRF(R_SKGPRF_EUFCMA(A), SKG_PRF.O_PRF_Default).main(true) @ &m : res]
+    - Pr[SKG_PRF.PRF(R_SKGPRF_EUFCMA(A), SKG_PRF.O_PRF_Default).main(false) @ &m : res] |
+  +
+  Pr[MCO_ITSR.ITSR(R_EUFCMA_ITSR(R_MFORSTWESNPRFEUFCMA_EUFCMA(A)), MCO_ITSR.O_ITSR_Default).main() @ &m : res]
+  +
+  Pr[FC_OpenPRE.SM_DT_OpenPRE_C(R_EUFCMA_FSMDTOpenPREC(R_MFORSTWESNPRFEUFCMA_EUFCMA(A)), FC_OpenPRE.O_SMDTOpenPRE_Default, FC.O_THFC_Default).main() @ &m : res]
+  +
+  Pr[FC_TCR.SM_DT_TCR_C(R_EUFCMA_FSMDTTCRC(R_MFORSTWESNPRFEUFCMA_EUFCMA(A)), FC_TCR.O_SMDTTCR_Default, FC.O_THFC_Default).main() @ &m : res]
+  + 
+  Pr[TRHC_TCR.SM_DT_TCR_C(R_EUFCMA_TRHSMDTTCRC(R_MFORSTWESNPRFEUFCMA_EUFCMA(A)), TRHC_TCR.O_SMDTTCR_Default, TRHC.O_THFC_Default).main() @ &m : res]
+  +
+  Pr[TRCOC_TCR.SM_DT_TCR_C(R_EUFCMA_TRCOSMDTTCRC(R_MFORSTWESNPRFEUFCMA_EUFCMA(A)), TRCOC_TCR.O_SMDTTCR_Default, TRCOC.O_THFC_Default).main() @ &m : res]  
+  +
+  (w - 2)%r
+    * `|Pr[FC_UD.SM_DT_UD_C(R_SMDTUDC_Game23WOTSTWES(R_MEUFGCMAWOTSTWESNPRF_EUFNACMA(R_FLSLXMSSMTTWESNPRFEUFNACMA_EUFCMA(A))), FC_UD.O_SMDTUD_Default, FC.O_THFC_Default).main(false) @ &m : res]
+        - Pr[FC_UD.SM_DT_UD_C(R_SMDTUDC_Game23WOTSTWES(R_MEUFGCMAWOTSTWESNPRF_EUFNACMA(R_FLSLXMSSMTTWESNPRFEUFNACMA_EUFCMA(A))), FC_UD.O_SMDTUD_Default, FC.O_THFC_Default).main(true) @ &m : res]| 
+  + 
+  Pr[FC_TCR.SM_DT_TCR_C(R_SMDTTCRC_Game34WOTSTWES(R_MEUFGCMAWOTSTWESNPRF_EUFNACMA(R_FLSLXMSSMTTWESNPRFEUFNACMA_EUFCMA(A))), FC_TCR.O_SMDTTCR_Default, FC.O_THFC_Default).main() @ &m : res] 
+  + 
+  Pr[FC_PRE.SM_DT_PRE_C(R_SMDTPREC_Game4WOTSTWES(R_MEUFGCMAWOTSTWESNPRF_EUFNACMA(R_FLSLXMSSMTTWESNPRFEUFNACMA_EUFCMA(A))), FC_PRE.O_SMDTPRE_Default, FC.O_THFC_Default).main() @ &m : res]
+  +
+  Pr[PKCOC_TCR.SM_DT_TCR_C(R_SMDTTCRCPKCO_EUFNACMA(R_FLSLXMSSMTTWESNPRFEUFNACMA_EUFCMA(A)), PKCOC_TCR.O_SMDTTCR_Default, PKCOC.O_THFC_Default).main() @ &m : res]
+  +
+  Pr[TRHC_TCR.SM_DT_TCR_C(R_SMDTTCRCTRH_EUFNACMA(R_FLSLXMSSMTTWESNPRFEUFNACMA_EUFCMA(A)), TRHC_TCR.O_SMDTTCR_Default, TRHC.O_THFC_Default).main() @ &m : res].
 proof. admit. qed.
-    
+ 
 end section Proof_SPHINCS_PLUS_TW_EUFCMA.
